theories/common/LanguagesCommon.v
@@ -124,3 +124,11 @@ Proof.
   - apply var_eqb_neq in Heq. right. assumption.
 Qed.
 
+Lemma triple_dec : forall (x y z : variable),
+  x = y \/
+  x = z \/
+  (x <> y /\ x <> z).
+Proof.
+intros x y z.
+  destruct (var_eqb_dec x y); destruct (var_eqb_dec x z); auto.
+Qed.
